sir/Sir/Theorems/Machine.lean
@@ -1,0 +1,1 @@
+import Sir.Spec.Machine
